SL/StoreHeapModel.thy
@@ -22,20 +22,17 @@ definition mutation :: "'s nat_exp \<Rightarrow> 's nat_exp \<Rightarrow> 's ptr
   "mutation e t \<equiv> \<langle>\<lambda>(s, h). if e s \<in> dom h
                             then Some (s, h(e s \<mapsto> t s))
                             else None\<rangle>"
-(*
-definition cons :: "(nat, 's) lval \<Rightarrow> 's nat_exp \<Rightarrow> 's ptran" where
-  "cons u_upd t \<equiv> \<langle>\<lambda>(s, h). let N = (SOME n. \<forall>x \<in> dom h. n > x) in
-                    Some (u_upd (\<lambda>_. N) s, h(N \<mapsto> t s))\<rangle>"
-*)
 
-definition cons :: "(nat, 's) lval \<Rightarrow> 's nat_exp \<Rightarrow> 's ptran" where
-  "cons u_upd t \<equiv> \<langle>\<lambda>(s, h). let N = (SOME n. n \<notin> dom h) in
+definition alloc :: "(nat, 's) lval \<Rightarrow> 's nat_exp \<Rightarrow> 's ptran" where
+  "alloc u_upd t \<equiv> \<langle>\<lambda>(s, h). let N = (SOME n. n \<notin> dom h) in
                     Some (u_upd (\<lambda>_. N) s, h ++ [N \<mapsto> t s])\<rangle>"
 
-definition dispose :: "'s nat_exp \<Rightarrow> 's ptran" where
-  "dispose e \<equiv> \<langle>\<lambda>(s, h). if e s \<in> dom h 
+definition disposal :: "'s nat_exp \<Rightarrow> 's ptran" where
+  "disposal e \<equiv> \<langle>\<lambda>(s, h). if e s \<in> dom h 
                          then Some (s, h(e s := None)) 
                          else None\<rangle>"
+
+(***********************************************************************************************)
 
 (* Monotonic *)
 
@@ -54,11 +51,13 @@ lemma mono_lookup [mptran]: "mono (lookup u t)"
 lemma mono_mutation [mptran]: "mono (mutation e t)"
   by (auto simp: mutation_def intro: mptran)
 
-lemma mono_cons [mptran]: "mono (cons u t)"
-  by (auto simp: cons_def intro: mptran)
+lemma mono_alloc [mptran]: "mono (alloc u t)"
+  by (auto simp: alloc_def intro: mptran)
 
-lemma mono_dispose [mptran]: "mono (dispose e)"
-  by (auto simp: dispose_def intro: mptran)
+lemma mono_disposal [mptran]: "mono (disposal e)"
+  by (auto simp: disposal_def intro: mptran)
+
+(***********************************************************************************************)
 
 (* Locality *)
 
@@ -88,23 +87,17 @@ lemma local_mutation [lptran]: "local (mutation e t) R"
   apply (auto simp: ortho_def)
 done
 
-lemma "Q n \<Longrightarrow> P (SOME n. Q n) \<Longrightarrow> P n"
-nitpick oops
-
-find_theorems name: ex_new_if_finite
-
 lemma "dom h \<noteq> UNIV \<Longrightarrow> \<exists>n. n \<notin> dom h"
   apply auto
 done
 
-lemma local_cons [lptran]: "\<forall>h. \<exists>n. n \<notin> dom h \<Longrightarrow> local (cons u t) R"
-apply (simp add: cons_def local_eq basic_local_def)
-apply auto
+lemma local_alloc [lptran]: "\<forall>h. \<exists>n. n \<notin> dom h \<Longrightarrow> local (alloc u t) R"
+  apply (simp add: alloc_def local_eq basic_local_def)
+  apply auto
 oops
 
-
-lemma local_dispose [lptran]: "local (dispose e) R"
-  apply (simp add: dispose_def local_def ortho_def sep_def basic_def valid_mem_def)
+lemma local_disposal [lptran]: "local (disposal e) R"
+  apply (simp add: disposal_def local_def ortho_def sep_def basic_def valid_mem_def)
   apply auto
   apply (erule_tac x="h1(e s := None)" in allE)
   apply auto 
@@ -117,6 +110,7 @@ lemma local_dispose [lptran]: "local (dispose e) R"
   apply (metis disjoint_iff_not_equal domI domIff fun_upd_apply option.case_eq_if)
   by (metis fun_upd_apply)
 
+(***********************************************************************************************)
 
 (* Separation Logic *)
 
@@ -126,6 +120,8 @@ lemma hl_basic [sl]: "P \<subseteq> {s. f s in Q} \<Longrightarrow> ht P (basic 
 lemma hl_assign [sl]: "P \<subseteq> subst_pred Q z_upd t \<Longrightarrow> ht P (assign z_upd t) Q"
   by (auto simp: assign_def subst_pred_def valid_mem_def intro!: sl)
 
+(* Mutation *)
+
 lemma sl_mut_local [sl]: "ht (e \<mapsto> -) (mutation e e') (e \<mapsto> e')"
   by (auto simp: mutation_def valid_mem_def any_singleton_def singleton_def intro!: sl)
 
@@ -133,59 +129,51 @@ lemma sl_mut_local' [sl]: "ht (e \<mapsto> n) (mutation e e') (e \<mapsto> e')"
   by (auto simp: mutation_def valid_mem_def any_singleton_def singleton_def intro!: sl)
 
 lemma sl_mut_global [sl]: "ht ((e \<mapsto> -) * r) (mutation e e') ((e \<mapsto> e') * r)"
-  by (auto intro: sl lptran)
+  by (auto intro: sl lptran sl_frame)
+
+lemma sl_mut_global' [sl]: "ht ((e \<mapsto> n) * r) (mutation e e') ((e \<mapsto> e') * r)"
+  by (auto intro: sl lptran sl_frame)
 
 lemma sl_mut: "ht ((e \<mapsto> -) * ((e \<mapsto> e') -* r)) (mutation e e') r"
   apply (rule hl_post[where Q'="(e \<mapsto> e') * ((e \<mapsto> e') -* r)"])
   by (auto simp: Assertions.bbi.sep_impl_annil1 intro!: sl_mut_global mptran)
 
-lemma sl_mut': "ht ((e \<mapsto> n) * ((e \<mapsto> e') -* r)) (mutation e e') r"
-sorry
+lemma sl_mut_suc [sl]: "ht (v \<mapsto> a, b) (mutation (\<lambda>s. v s + 1) e) (v \<mapsto> a, e)"
+  by (auto simp add: doublet_def intro: sl_frame2 lptran sl)
 
-lemma sl_dipose_local [sl]: "ht (e \<mapsto> -) (dispose e) (emp)"
-  by (auto simp: dispose_def singleton_def valid_mem_def any_singleton_def emp_def intro!: sl)
+(* Allocation *)
 
-lemma sl_dispose [sl]: "ht ((e \<mapsto> -) * r) (dispose e) r"
-  by (subst bbi.mult_1[symmetric], (rule sl | rule lptran)+)
+lemma sl_alloc_local [sl]: "free u_upd e \<Longrightarrow> vars1 u_upd u \<Longrightarrow> ht emp (alloc u_upd e) (u \<mapsto> e)"
+  apply (auto simp: alloc_def emp_def valid_mem_def singleton_def intro!: sl)
+  apply (case_tac "let N = SOME n. True in Some (u_upd (\<lambda>_. N) a, [N \<mapsto> e a])")
+  apply (metis option.distinct(1))
+  apply (auto simp add: Let_unfold)
+done
 
-lemma sl_dispose_alt [sl]: "ht ((e \<mapsto> n) * r) (dispose e) r"
+(* Disposal *)
+
+lemma sl_dipose_local [sl]: "ht (e \<mapsto> -) (disposal e) (emp)"
+  by (auto simp: disposal_def singleton_def valid_mem_def any_singleton_def emp_def intro!: sl)
+
+lemma sl_disposal [sl]: "ht ((e \<mapsto> -) * r) (disposal e) r"
+  by (subst bbi.mult_1[symmetric], (rule sl | rule lptran | rule sl_frame)+)
+
+lemma sl_disposal_alt [sl]: "ht ((e \<mapsto> n) * r) (disposal e) r"
   apply (rule hl_pre)
   defer
-  apply (rule sl_dispose)
+  apply (rule sl_disposal)
   apply (rule bbi.qiso)
   by (auto simp: any_singleton_def singleton_def)
 
-lemma sl_alloc_local [sl]: "free u_upd e \<Longrightarrow> vars1 u_upd u \<Longrightarrow> ht emp (cons u_upd e) (u \<mapsto> e)"
-  apply (auto simp: cons_def emp_def valid_mem_def singleton_def intro!: sl)
-  apply (case_tac "let N = SOME n. True in Some (u_upd (\<lambda>_. N) a, [N \<mapsto> e a])")
-  apply (metis option.distinct(1))
-  apply clarsimp
-  apply (simp add: Let_unfold)
-  apply auto
-done
+(* Lookup *)
 
-lemma sl_alloc_global [sl]: "free u_upd e \<Longrightarrow> vars1 u_upd u \<Longrightarrow> ht r (cons u_upd e) ((u \<mapsto> e) * r)"
-  oops
-
-lemma sl_alloc  [sl]: "free u_upd e \<Longrightarrow> free_pred u_upd r \<Longrightarrow> ht (ALLS v. (v \<mapsto> e) -* r) (cons u_upd e) r"
-  oops
-
-lemma sl_lookup_local [sl]: "vars2 v_upd v v' \<Longrightarrow> vars3 v_upd v' \<Longrightarrow> free v_upd e \<Longrightarrow> 
+lemma sl_lookup_local: "vars2 v_upd v v' \<Longrightarrow> vars3 v_upd v' \<Longrightarrow> free v_upd e \<Longrightarrow> 
     ht (e \<mapsto> v') (lookup v_upd e) ((v \<Midarrow> v') \<sqinter> (e \<mapsto> v'))"
   by (auto simp: lookup_def valid_mem_def singleton_def intro!: sl)
 
-lemma sl_lookup_global [sl]: "vars2 v_upd v v' \<Longrightarrow> vars3 v_upd v' \<Longrightarrow> free v_upd e \<Longrightarrow> 
-    ht ((e \<mapsto> v') * r) (lookup v_upd e) ((<{s. v s = v' s}> * (e \<mapsto> v')) * r)"
-oops
-
-lemma sl_lookup_lkl [sl]: "vars1 v_upd v \<Longrightarrow> vars3 v_upd v'' \<Longrightarrow> free v_upd e \<Longrightarrow>
+lemma sl_lookup_lkl: "vars1 v_upd v \<Longrightarrow> vars3 v_upd v'' \<Longrightarrow> free v_upd e \<Longrightarrow>
     ht ((v \<Midarrow> v') \<sqinter> (e \<mapsto> v'')) (lookup v_upd e) ((v \<Midarrow> v'') \<sqinter> (subst e v_upd v' \<mapsto> v))"
   by (auto simp: lookup_def valid_mem_def singleton_def intro!: sl)
-
-lemma lookup_ref45:"ht (EXS x. (e \<mapsto> (\<lambda>_. x)) * R (\<lambda>_. x)) (lookup k_update e) ((e \<mapsto> k) * R k)"
-sorry
-
-
 
 lemma sl_lookup: "ht (EXS v'. (e \<mapsto> v') * ((e \<mapsto> v') -* (subst_pred r v_upd v'))) (lookup v_upd e) r"
   apply (auto simp: lookup_def intro!: sl)
@@ -205,7 +193,7 @@ lemma sl_lookup: "ht (EXS v'. (e \<mapsto> v') * ((e \<mapsto> v') -* (subst_pre
   apply auto
   by (simp add: domI ortho_def)
 
-lemma sl_lookup2: "ht (EXS v'. (e \<mapsto> $v') * ((e \<mapsto> $v') -* (subst_pred r v_upd $v'))) (lookup v_upd e) r"
+lemma sl_lookup': "ht (EXS v'. (e \<mapsto> $v') * ((e \<mapsto> $v') -* (subst_pred r v_upd $v'))) (lookup v_upd e) r"
   apply (auto simp: lookup_def intro!: sl)
   apply (subgoal_tac "(a, b) \<in> subst_pred r v_upd $x")
   prefer 2
@@ -240,7 +228,7 @@ lemma sl_lookup_alt: "ht (EXS v'. (e \<hookrightarrow> v') \<sqinter> (subst_pre
   apply (rule reynolds6)
 done
 
-lemma sl_lookup_alt2: "ht (EXS v'. (e \<hookrightarrow> $v') \<sqinter> (subst_pred r v_upd $v')) (lookup v_upd e) r"
+lemma sl_lookup_alt' [sl]: "ht (EXS v'. (e \<hookrightarrow> $v') \<sqinter> (subst_pred r v_upd $v')) (lookup v_upd e) r"
   apply (rule hl_pre)
   prefer 2
   apply (rule sl_lookup)
@@ -257,17 +245,65 @@ lemma sl_lookup_alt2: "ht (EXS v'. (e \<hookrightarrow> $v') \<sqinter> (subst_p
   apply (rule reynolds6)
 done
 
-lemma sl_lookup_alt3: "p \<subseteq> (EXS v'. (e \<hookrightarrow> $v') \<sqinter> (subst_pred q v_upd $v')) \<Longrightarrow> ht p (lookup v_upd e) q"
-apply (rule hl_pre)
-apply assumption
-apply (rule sl_lookup_alt2)
+lemma sl_lookup_var: "p \<subseteq> (EXS v'. (e \<hookrightarrow> $v') \<sqinter> (subst_pred q v_upd $v')) \<Longrightarrow> ht p (lookup v_upd e) q"
+  apply (rule hl_pre)
+  apply assumption
+  apply (rule sl_lookup_alt')
 done
 
-lemma lookup_ref452 [sl]:"ht (EXS x. (v \<mapsto> (\<lambda>_. a), (\<lambda>_. x)) * R (\<lambda>_. x)) (lookup k_upd (\<lambda>s. v s + 1)) ((v \<mapsto> b, kei) * R kei)"
-sorry
+lemma lookup_suc_ref [sl]:"\<forall>x s. v (k_upd (\<lambda>_. x) s) = v s \<Longrightarrow> \<forall>x s. k (k_upd (\<lambda>_. x) s) = x \<Longrightarrow> 
+  \<forall>x. subst_pred (R k) k_upd (\<lambda>_. x) = R (\<lambda>_. x) \<Longrightarrow> 
+  ht (EXS x. (v \<mapsto> (\<lambda>_. a), (\<lambda>_. x)) * R (\<lambda>_. x)) (lookup k_upd (\<lambda>s. v s + 1)) ((v \<mapsto> (\<lambda>_. a), k) * R k)"
+  apply (rule hl_classic)
+  apply (rule mptran)+
+  defer
+  defer
+  apply (rule sl_lookup_alt')
+  defer
+  apply (rule subset_refl)
+  apply (rule mono_exs)
+  apply (simp add: doublet_def)
+  apply (rule conjI)
+  apply (simp add: points_to_def)
+  apply (metis (no_types, lifting) Assertions.bbi.intuitionistic_sep_conj_top Assertions.bbi.intuitionistic_sep_impl_closure Assertions.bbi.intuitionistic_top Assertions.bbi.sep_impl_annir2 Assertions.bbi.sep_impl_isoE Assertions.bbi.sep_impl_top_x Assertions.bbi.strongest_intuitionistic sep_comm top_greatest)
+  apply (subst spred)+
+  apply simp
+done
 
-lemma mutation_ref452 [sl]: "ht (v \<mapsto> a, b) (mutation (\<lambda>s. v s + 1) e) (v \<mapsto> a, e)"
-  sorry
+lemma lookup_suc_ref':"\<forall>x s. v (k_upd (\<lambda>_. x) s) = v s \<Longrightarrow> \<forall>x s. k (k_upd (\<lambda>_. x) s) = x \<Longrightarrow> 
+  \<forall>x. subst_pred (R k) k_upd (\<lambda>_. x) = R (\<lambda>_. x) \<Longrightarrow> 
+  ht (EXS x. (v \<mapsto> (\<lambda>_. a), (\<lambda>_. x)) * R (\<lambda>_. x)) (lookup k_upd (\<lambda>s. v s + 1)) ((v \<mapsto> -) * (((\<lambda>s. v s + 1) \<mapsto> -) * R k))"
+  apply (rule hl_classic)
+  apply (rule mptran)+
+  defer
+  defer
+  apply (rule sl_lookup_alt')
+  defer
+  apply (rule subset_refl)
+  apply (rule mono_exs)
+  apply (simp add: doublet_def)
+  apply (rule conjI)
+  apply (simp add: points_to_def)
+  apply (metis (no_types, lifting) Assertions.bbi.intuitionistic_sep_conj_top Assertions.bbi.intuitionistic_sep_impl_closure Assertions.bbi.intuitionistic_top Assertions.bbi.sep_impl_annir2 Assertions.bbi.sep_impl_isoE Assertions.bbi.sep_impl_top_x Assertions.bbi.strongest_intuitionistic sep_comm top_greatest)
+  apply (subst spred)+
+  apply simp
+  apply sep_auto
+done
+
+lemma lookup_suc_var_ref [sl]:"\<forall>x s. v (k_upd (\<lambda>_. x) s) = v s \<Longrightarrow> \<forall>x s. k (k_upd (\<lambda>_. x) s) = x \<Longrightarrow> 
+  \<forall>x. subst_pred (R k) k_upd (\<lambda>_. x) = R (\<lambda>_. x) \<Longrightarrow> P \<le> (EXS x. (v \<mapsto> (\<lambda>_. a), (\<lambda>_. x)) * R (\<lambda>_. x)) \<Longrightarrow> 
+  ht P (lookup k_upd (\<lambda>s. v s + 1)) ((v \<mapsto> -) * (((\<lambda>s. v s + 1) \<mapsto> -) * R k))"
+  apply (rule hl_pre)
+  defer
+  apply (rule lookup_suc_ref')
+  apply simp+
+done
+
+no_notation basic ("\<langle>_\<rangle>")
+
+(***********************************************************************************************)
+
+(* Hoare tactic *)
 
 named_theorems hl_rules
 
