Algebra/DomainSeparationSemiring.thy
@@ -1,0 +1,19 @@
+theory DomainSeparationSemiring
+  imports "KAD/Domain_Semiring"
+begin
+
+no_notation times (infixl "*" 70)
+
+class dss_no_loc = antidomain_semiring +
+  fixes sep :: "'a \<Rightarrow> 'a \<Rightarrow> 'a" (infixl "*" 55)
+  and e :: 'a
+  assumes dss1: "d(d x * d y) = d x * d y"  
+  and dss2: "d(x * (y * z)) = d ((x * y) * z)"  
+  and dss3: "d(x * (y + z)) = d (x * y) + d (x * z)"  
+  and dss4: "d(x * y) = d (y * x)"  
+  and dss5: "d(x * e) = d x"  
+
+class dss = dss_no_loc +
+  assumes loc: "d(x \<cdot> (y * z)) \<le> d ((x \<cdot> y) * z)"  
+
+end
