Algebra/KAD/Separation_Semiring.thy
@@ -1,0 +1,218 @@
+theory Separation_Semiring
+  imports Domain_Semiring Range_Semiring
+begin
+
+no_notation
+  fdiamond ("\<bar> _ \<rangle> _" [50,90] 95) and
+  fbox ("\<bar> _ ] _" [50,90] 95) and
+  bdiamond ("\<langle> _ \<bar> _" [50,90] 95) and
+  bbox ("[ _ \<bar> _" [50,90] 95) and
+  times (infixl "*" 70)
+
+context antidomain_semiring
+begin
+
+definition fdia :: "'a \<Rightarrow> 'a \<Rightarrow> 'a" ("\<bar>_\<rangle>_" [99, 99] 100) where
+  "\<bar>x\<rangle>y = d(x\<cdot>y)"
+  
+definition fbox :: "'a \<Rightarrow> 'a \<Rightarrow> 'a" ("\<bar>_]_" [99, 99] 100) where
+  "\<bar>x]y = a( \<bar>x\<rangle> a(y) )"
+
+lemma fbox_def_var: "\<bar>x]y = a(x\<cdot>a(y))"
+  by (metis fdia_def fbox_def local.a_5)
+  
+sublocale fmodal: fmodal_semiring where fdiamond = fdia and fbox = fbox
+  apply default
+  apply (simp_all add: fdia_def fbox_def_var)
+done
+  
+lemma fswap: "p = d(p) \<Longrightarrow> q = d(q) \<Longrightarrow> \<bar>x\<rangle>p \<le> \<bar>y]q \<longleftrightarrow> \<bar>y\<rangle>a(q) \<le> \<bar>x]a(p)"
+  by (metis local.a_antitone local.antidomain_semiring_domain_def local.fmodal.fbox_fdia_de_morgan_1 local.fmodal.fdia_fbox_de_morgan_2)
+
+end
+
+interpretation rel: antidomain_semiring "op \<union>" "op O" Id "{}" "\<lambda>x. -(Id \<inter> x O UNIV) \<inter> Id" "op \<subseteq>" "op \<subset>"
+apply default
+apply auto
+by (metis ComplI IdI Int_iff UNIV_I compl_inf relcomp.simps)
+
+interpretation rel: antirange_semiring "op \<union>" "op O" Id "{}" "\<lambda>x. -(Id \<inter> UNIV O x) \<inter> Id" "op \<subseteq>" "op \<subset>"
+apply default
+apply auto
+by (metis ComplI IdI Int_iff UNIV_I compl_inf relcomp.simps)
+
+class sepconj =
+  fixes sepconj :: "'a \<Rightarrow> 'a \<Rightarrow> 'a" (infixl "*" 80)
+  and sepunit :: "'a" ("e")
+  
+class ss_domain = antidomain_semiring + sepconj +
+  assumes d6: "d(d(x) * d(y)) = d(x) * d(y)"
+  and d7: "d(x * (y * z)) = d((x * y) * z)"
+  and d8: "d(x * (y + z)) = d(x * y) + d(x * z)"
+  and d9: "d(x * y) = d(y * x)"
+  and d10: "d(x * e) = d(x)"
+  and d_loc: "d(x \<cdot> (y * z)) \<le> d(x\<cdot>y) * d(z)"
+begin
+
+lemma d_loc': "d p = p \<Longrightarrow> d q = q \<Longrightarrow> d(x \<cdot> (p * q)) \<le> d(x\<cdot>p) * q"
+  by (metis local.d_loc)
+
+lemma fdia_local: "d(p) = p \<Longrightarrow> d(q) = q \<Longrightarrow> \<bar>x\<rangle>(p * q) \<le> \<bar>x\<rangle>p * q"
+  by (metis local.d_loc' local.fmodal.fdiamond_def)
+  
+lemma fbox_local: "\<lbrakk>p = d(p); q = d(q)\<rbrakk> \<Longrightarrow> \<bar>x]p * q \<le> \<bar>x](p * q)"
+  (* nitpick *) oops
+
+end
+
+context antirange_semiring
+begin
+
+definition bdia :: "'a \<Rightarrow> 'a \<Rightarrow> 'a" ("\<langle>_\<bar>_" [99, 99] 100) where
+  "\<langle>x\<bar>y = r(y\<cdot>x)"
+  
+definition bbox :: "'a \<Rightarrow> 'a \<Rightarrow> 'a" ("[_\<bar>_" [99, 99] 100) where
+  "[x\<bar>y = ar( \<langle>x\<bar> ar(y) )"
+
+lemma bbox_def_var: "[x\<bar>y = ar(ar(y)\<cdot>x)"
+  by (metis bdia_def local.antirange_semiring_range_def local.bbox_def local.dual.a_closure local.dual.antidomain_semiring_domain_def)
+  
+sublocale bmodal: bmodal_semiring where bdiamond = bdia and bbox = bbox
+  apply default
+  apply (simp_all add: bdia_def bbox_def_var)
+done
+
+lemma bswap: "p = r(p) \<Longrightarrow> q = r(q) \<Longrightarrow> \<langle>x\<bar>p \<le> [y\<bar>q \<longleftrightarrow> \<langle>y\<bar>ar(q) \<le> [x\<bar>ar(p)"
+  by (metis local.bmodal.dual.fbox_fdia local.bmodal.dual.fdia_fbox_de_morgan_2 local.bmodal.dual.fdia_simp_2 local.dual.a_antitone local.dual.antidomain_semiring_domain_def)
+
+end
+
+class ss_range = antirange_semiring + sepconj +
+  assumes r6: "r(r(x) * r(y)) = r(x) * r(y)"
+  and r7: "r(x * (y * z)) = r((x * y) * z)"
+  and r8: "r(x * (y + z)) = r(x * y) + r(x * z)"
+  and r9: "r(x * y) = r(y * x)"
+  and r10: "r(x * e) = r(x)"
+  and r_loc: "r((x * y) \<cdot> z) \<le> r(x\<cdot>z) * r(y)"
+begin
+
+lemma bdia_local: "r(p) = p \<Longrightarrow> r(q) = q \<Longrightarrow> \<langle>x\<bar>(p * q) \<le> \<langle>x\<bar>p * q"
+  by (metis local.r_loc bdiamond_def)
+
+end
+
+class modal_semiring = antidomain_semiring + antirange_semiring +
+  assumes domrange: "d(r(x))=r(x)"
+  and rangedom: "r(d(x))=d(x)"
+begin
+
+lemma domrangefix: "d(x)=x \<longleftrightarrow> r(x)=x"
+  by (metis domrange rangedom)
+
+lemma box_diamond_galois_1: "\<lbrakk>p=d(p); q=d(q)\<rbrakk> \<Longrightarrow> (\<langle>x\<bar>p \<le> q \<longleftrightarrow> p \<le> \<bar>x]q)"
+  by (metis domrangefix fbox_demodalisation3 rdemodalisation3)
+  
+lemma box_diamond_galois_2: "\<lbrakk>p=d(p); q=d(q)\<rbrakk> \<Longrightarrow> ( \<bar>x\<rangle>p \<le> q \<longleftrightarrow> p \<le> [x\<bar>q)"
+  by (metis domrangefix bbox_demodalisation3 fdemodalisation3)
+
+lemma diamond_conjugation_var_1: "\<lbrakk>p=d(p); q=d(q)\<rbrakk> \<Longrightarrow>( \<bar>x\<rangle>q \<le> a(p) \<longleftrightarrow> \<langle>x\<bar>p \<le> a(q))"
+  by (smt a_closure a_export antidomain_semiring_domain_def box_diamond_galois_1 domain_1 fbox_def fdia_fbox less_eq_def)
+
+lemma diamond_conjugation: "\<lbrakk>p=d(p); q=d(q)\<rbrakk> \<Longrightarrow> (p\<cdot>( \<bar>x\<rangle>q) = 0 \<longleftrightarrow> q\<cdot>(\<langle>x\<bar>p) = 0)" 
+  by (metis diamond_conjugation_var_1 fdia_simp_2 bdia_simp_2 domrange d_d_zero dom_el_comm)
+
+lemma box_conjugation:  "\<lbrakk>p=d(p); q=d(q)\<rbrakk> \<Longrightarrow> (p \<le> [x\<bar>a(q) \<longleftrightarrow> q \<le> \<bar>x]a(p))"
+  by (metis box_diamond_galois_2 a_closure diamond_conjugation_var_1  box_diamond_galois_1 antidomain_semiring_domain_def)
+
+lemma box_diamond_cancellation_1:  "p=d(p)  \<Longrightarrow>  p \<le> \<bar>x](\<langle>x\<bar>p)"
+  by (metis bdiamond_def box_diamond_galois_1 domrange order_refl)
+
+lemma box_diamond_cancellation_2:  "p=d(p)  \<Longrightarrow>  p \<le> [x\<bar>( \<bar>x\<rangle>p)"
+  by (metis box_diamond_galois_2 domain_invol fdiamond_def order_refl)
+
+lemma box_diamond_cancellation_3:  "q=d(q) \<Longrightarrow> \<bar>x\<rangle>([x\<bar>q) \<le> q"
+  by (metis ar_closure box_diamond_galois_2 domrangefix dual.fbox_fdia order_refl)
+
+lemma box_diamond_cancellation_4:  "q=d(q) \<Longrightarrow> \<langle>x\<bar>( \<bar>x]q) \<le> q"
+  by (metis a_closure box_diamond_galois_1 fbox_def order_refl) 
+  
+lemma antidomran: "d(x) = x \<Longrightarrow> a(x) = ar(x)"
+  by (metis local.a_gla local.antidomain_semiring_domain_def local.antirange_semiring_range_def local.antisym_conv local.ar1 local.ar_gla local.domrange local.rangedom)  
+
+end
+
+interpretation rel: modal_semiring "op \<union>" "op O" Id "{}" "\<lambda>x. -(Id \<inter> x O UNIV) \<inter> Id" "op \<subseteq>" "op \<subset>" "\<lambda>x. -(Id \<inter> UNIV O x) \<inter> Id"
+  apply default
+  apply (subst rel.antidomain_semiring_domain_def)
+  apply (subst rel.antirange_semiring_range_def)+
+  prefer 2
+  apply (subst rel.antidomain_semiring_domain_def)+
+  apply (subst rel.antirange_semiring_range_def)
+  apply force
+  apply fastforce
+done
+
+
+class modal_separation_semiring = modal_semiring + ss_domain + ss_range 
+begin
+
+lemma dsep_isol: "d(y) \<le> d(z) \<Longrightarrow> d(x) * d(y) \<le> d(x) * d(z)"
+proof (simp add: less_eq_def)
+  assume assms: "d y + d z = d z"
+  have "d x * d y + d x * d z = d (d x * d y) + d(d x * d z)"
+    by (metis d6)
+  also have "... = d (d x * (d y + d z))"
+    by (metis d8)
+  also have "... = d (d x * d z)"
+    by (metis assms)
+  finally show "d x * d y + d x * d z = d x * d z"
+    by (metis d6)
+qed
+
+lemma dsep_isor: "d(x) \<le> d(y) \<Longrightarrow> d(x) * d(z) \<le> d(y) * d(z)"
+  using dsep_isol local.d6 local.d9 by smt
+  
+lemma dsep_isol_var: "p=d(p) \<Longrightarrow> q=d(q) \<Longrightarrow> s=d(s) \<Longrightarrow> p \<le> q \<Longrightarrow> s * p \<le> s * q"
+  by (metis dsep_isol)
+
+lemma dsep_isor_var: "p=d(p) \<Longrightarrow> q=d(q) \<Longrightarrow> s=d(s) \<Longrightarrow> p \<le> q \<Longrightarrow> p * s \<le> q * s"
+  by (metis dsep_isor)
+
+lemma d_sepconj: "d(p) = p \<Longrightarrow> d(q) = q \<Longrightarrow> d(p * q) = p * q"
+  by (metis local.d6)
+  
+lemma fbox_local: "\<lbrakk>p = d(p); q = d(q)\<rbrakk> \<Longrightarrow> \<bar>x]p * q \<le> \<bar>x](p * q)"
+proof -
+  assume tests:"p = d(p)" "q = d(q)"
+  hence "\<langle>x\<bar>(\<bar>x]p * q) \<le> \<langle>x\<bar>(\<bar>x]p) * q"
+    by (metis bdia_local local.fmodal.fbox_simp_2 domrangefix)
+  moreover have "\<langle>x\<bar>(\<bar>x]p) \<le> p"
+    by (metis local.box_diamond_cancellation_4 tests(1))
+  ultimately have "\<langle>x\<bar>(\<bar>x]p * q) \<le> p * q"
+    apply (subst tests(1))
+    apply (rule dual_order.trans)
+    using tests apply (auto intro!: dsep_isor_var)
+    by (metis local.antirange_semiring_range_def local.bmodal.dual.fdia_simp_2 local.domrangefix local.dual.antidomain_semiring_domain_def)
+  thus ?thesis
+    by (metis local.box_diamond_galois_1 local.d6 local.fmodal.fbox_simp_2 tests(1) tests(2))
+qed
+
+lemma bbox_local: "\<lbrakk>p = d(p); q = d(q)\<rbrakk> \<Longrightarrow> [x\<bar>p * q \<le> [x\<bar>(p * q)"
+proof -
+  assume tests:"p = d(p)" "q = d(q)"
+  hence "\<bar>x\<rangle>([x\<bar>p * q) \<le> \<bar>x\<rangle>([x\<bar>p) * q"
+    by (metis local.d_loc local.fmodal.fdiamond_def)
+  moreover have "\<bar>x\<rangle>([x\<bar>p) \<le> p"
+    by (metis local.box_diamond_cancellation_3 tests(1))
+  ultimately have "\<bar>x\<rangle>([x\<bar>p * q) \<le> p * q"
+    apply (subst tests(1))
+    apply (rule dual_order.trans)
+    using tests apply (auto intro!: dsep_isor_var)
+    by (metis local.fmodal.fdia_simp_2)
+  thus ?thesis
+    by (metis d_sepconj local.antirange_semiring_range_def local.bmodal.dual.fbox_fdia local.box_diamond_galois_2 local.domrangefix local.dual.a_closure local.dual.antidomain_semiring_domain_def tests(1) tests(2))
+qed
+
+end
+
+end
