SL/LinkedList.thy
@@ -96,7 +96,7 @@ lemmas [sep_simp] =
   llist_empty_zero
   llist_simp
 
-lemma zero: "(s, h) \<in> llist x i * R \<Longrightarrow> i s = 0 \<Longrightarrow> (x = [] \<Longrightarrow> (s, h) \<in> R \<Longrightarrow> Q) \<Longrightarrow> Q"
+lemma llist_emptyE: "(s, h) \<in> llist x i * R \<Longrightarrow> i s = 0 \<Longrightarrow> (x = [] \<Longrightarrow> (s, h) \<in> R \<Longrightarrow> Q) \<Longrightarrow> Q"
   apply (induct x)
   apply (simp add: llist_empty)
   apply (erule spE)
@@ -104,7 +104,7 @@ lemma zero: "(s, h) \<in> llist x i * R \<Longrightarrow> i s = 0 \<Longrightarr
   apply (simp add: llist_simp)
 by (metis (no_types, lifting) CollectD bbi.mult_assoc less_numeral_extra(3) spE)
 
-lemma not_zero: "(s, h) \<in> llist x i * R \<Longrightarrow> i s \<noteq> 0 \<Longrightarrow> (x \<noteq> [] \<Longrightarrow> (s, h) \<in> llist (Cons (hd x) (tl x)) i * R \<Longrightarrow> Q) \<Longrightarrow> Q"
+lemma llist_non_emptyE: "(s, h) \<in> llist x i * R \<Longrightarrow> i s \<noteq> 0 \<Longrightarrow> (x \<noteq> [] \<Longrightarrow> (s, h) \<in> llist (Cons (hd x) (tl x)) i * R \<Longrightarrow> Q) \<Longrightarrow> Q"
   apply (induct x)
   apply (simp add: llist_empty)
   apply (erule spE)
@@ -112,27 +112,73 @@ lemma not_zero: "(s, h) \<in> llist x i * R \<Longrightarrow> i s \<noteq> 0 \<L
   apply (simp add: llist_simp)
 done
 
-schematic_lemma llist_J: "(s, h) \<in> llist xa j \<Longrightarrow> (s, h) \<in> llist xa (\<lambda>_. ?x)"
-  apply (induct xa arbitrary: x)
-  apply (simp add: llist_empty store_pred_def)
-oops
-
-lemma final: "(s, h) \<in> llist xs j \<Longrightarrow> (s, h) \<in> llist xs (\<lambda>_. j s)"
+lemma llist_store_idepend: "(s, h) \<in> llist xs j \<Longrightarrow> (s, h) \<in> llist xs (\<lambda>_. j s)"
   apply (induct xs)
   apply (simp add: sep_simp llist_empty store_pred_def)
   apply (simp add: llist_simp)
   apply auto
-
-        apply (erule spE)
-        apply (erule pred_exE)
-        apply (rule_tac x=x in exI)
-        apply (simp add: singleton_def doublet_def sep_def)
-        apply (erule spE)
-        apply simp
+  apply (erule spE)
+  apply (erule pred_exE)
+  apply (rule_tac x=x in exI)
+  apply (simp add: singleton_def doublet_def sep_def)
+  apply (erule spE)
+  apply simp
 done
 
-declare zero [sep_elim]
-  not_zero [sep_safe_elim]
+lemma sepD: "(x, y) \<in> P * Q \<Longrightarrow> \<exists>y1 y2. y = y1 ++ y2 \<and> y1 \<bottom> y2 \<and> (x, y1) \<in> P \<and> (x, y2) \<in> Q"
+  by (auto simp: sep_def)
+
+lemma llist_emp: "i x = 0 \<Longrightarrow> (x, y) \<in> llist xa i \<Longrightarrow> (x, y) \<in> emp"
+  apply (simp add: llist_def)
+  apply (erule conjE)
+  apply (induct xa)
+  apply simp
+  apply simp
+  apply (erule exE)
+  apply (drule sepD)
+  apply (erule exE)+
+  apply (erule conjE)+
+  apply (simp add: doublet_def)
+  apply (drule sepD)
+  apply (erule exE)+
+  apply (erule conjE)+  
+  apply (simp add: singleton_def)
+done
+
+lemma llist_cons: "0 < i x \<Longrightarrow> (x, y) \<in> llist xa i \<Longrightarrow> \<exists>j. (x, y) \<in> (i \<mapsto> (\<lambda>s. hd xa)) * (((\<lambda>s. Suc (i s)) \<mapsto> (\<lambda>s. j)) * llist (tl xa) (\<lambda>s. j))"
+  apply (simp add: llist_def)
+  apply (erule conjE)
+  apply (induct xa)
+  apply simp
+  apply simp
+  apply (erule exE)
+  apply (simp add: doublet_def)
+  apply (rule_tac x=xb in exI)
+  apply sep_simp
+  apply sep_auto
+  apply force
+done
+
+lemma llist_cons_true: "0 < i x \<Longrightarrow> (x, y) \<in> llist xa i \<Longrightarrow> \<exists>j. (x, y) \<in> ((\<lambda>s. Suc (i s)) \<mapsto> (\<lambda>s. j)) * true"
+  apply (drule llist_cons) back
+  apply assumption
+  apply auto
+  apply (subst (asm) sep_assoc[symmetric])
+  apply (subst (asm) sep_comm)
+  apply sep_auto
+done
+
+lemma llist_cons_var: "0 < i x \<Longrightarrow> (x, y) \<in> llist xa i \<Longrightarrow> \<exists>xb xc xd. (x, y) \<in> (i \<mapsto> (\<lambda>s. xb)) * (((\<lambda>s. Suc (i s)) \<mapsto> (\<lambda>s. xc)) * llist xd (\<lambda>s. xc))"
+  apply (drule llist_cons) back
+  apply assumption
+  apply auto
+done
+
+
+declare llist_emptyE [sep_elim]
+  llist_non_emptyE [sep_safe_elim]
+  llist_emp [sep_elim]
+  llist_cons_var [intro]
   hd_tl [sep_intro]
-  final [intro]
+  llist_store_idepend [intro]
 end
