SL/ListReversal.thy
@@ -1,135 +1,143 @@
 theory ListReversal
-  imports LinkedList Refinement
+  imports LinkedList Syntax
 begin
 
 record rev_list =
   i :: nat
   j :: nat
   k :: nat
+ 
+no_notation pmult_one_class.pmult_one ("1")
 
-
-lemma "ht (list_seg (Cons x xs) i k)
-    (
-      lookup j_update (\<lambda>s. (i s) + 1);
-      dispose i;
-      dispose (\<lambda>s. i s + 1);
-      assign i_update j
-    )
-    (list_seg xs i k)"
-apply hoare 
-sorry
-
-lemma "spec (llist xs i) (llist (rev xs) j) \<le> (
-      assign j_update $0;
-      while ({(s, h). i s \<noteq> 0}) 
-        (
-          lookup k_update (\<lambda>s. i s + 1);
-          mutation (\<lambda>s. i s + 1) j;
-          assign j_update i;
-          assign i_update k
-        )
-      )"
+lemma "\<lbrakk>llist xs i, llist (rev xs) j\<rbrakk> \<le>
+      `j := 0;
+      while `i \<noteq> 0 do 
+        `k := @(`i + 1);
+        @(`i + 1) := `j;
+        `j := `i;
+        `i := `k
+      od"
 proof -
-  have "spec (llist xs i) (llist (rev xs) j) \<le>
-      assign j_update $0; 
-      (spec (EXS A B. llist A i * llist B j * <{s. rev xs = (rev A) @ B}>) (llist (rev xs) j))"
+  have "\<lbrakk>llist xs i, llist (rev xs) j\<rbrakk> \<le>
+      `j := 0; 
+      \<lbrakk>EXS A B. llist A i * llist B j * \<langle>rev xs = (rev A) @ B\<rangle>, llist (rev xs) j\<rbrakk>"
       by morgan (sep_auto, auto)
   also have "... \<le> 
-      assign j_update $0; 
-      while ({(s, h). i s \<noteq> 0})  (
-        (spec (EXS A B. llist A i * llist B j * <{s. rev xs = (rev A) @ B}> * <{s. i s \<noteq> 0}>)
-              (EXS A B. llist A i * llist B j * <{s. rev xs = (rev A) @ B}>))
-      )"
+      `j := 0; 
+      while `i \<noteq> 0 do 
+        \<lbrakk>EXS A B. llist A i * llist B j * \<langle>rev xs = (rev A) @ B\<rangle> * \<langle>`i \<noteq> 0\<rangle>,
+         EXS A B. llist A i * llist B j * \<langle>rev xs = (rev A) @ B\<rangle>\<rbrakk>
+      od"
       by morgan sep_auto+
   also have "... \<le> 
-      assign j_update $0; 
-      while ({(s, h). i s \<noteq> 0})  (
-        (spec (EXS A B a k. (i \<mapsto> $a, $k) * llist A $k * llist B j * <{s. rev xs = (rev (Cons a A)) @ B}> * <{s. i s \<noteq> 0}>)
-              (EXS A B. llist A i * llist B j * <{s. rev xs = (rev A) @ B}>))
-      )"
+      `j := 0; 
+      while `i \<noteq> 0 do 
+        \<lbrakk>EXS A B a k. (i \<mapsto> $a, $k) * llist A $k * llist B j * \<langle>rev xs = (rev (a#A)) @ B\<rangle> * \<langle>`i \<noteq> 0\<rangle>,
+         EXS A B. llist A i * llist B j * \<langle>rev xs = (rev A) @ B\<rangle>\<rbrakk>
+      od"
       by morgan (sep_safe, sep_auto)
   also have "... \<le> 
-      assign j_update $0; 
-      while ({(s, h). i s \<noteq> 0})  (
-        lookup k_update (\<lambda>s. i s + 1);
-        (spec (EXS A B a. (i \<mapsto> $a, k) * llist A k * llist B j * <{s. rev xs = (rev (Cons a A)) @ B}> * <{s. i s \<noteq> 0}>)
-              (EXS A B. llist A i * llist B j * <{s. rev xs = (rev A) @ B}>))
-      )"
+      `j := 0; 
+      while `i \<noteq> 0 do 
+        `k := @(`i + 1);
+        \<lbrakk>EXS A B a. (i \<mapsto> $a, k) * llist A k * llist B j * \<langle>rev xs = (rev (a#A)) @ B\<rangle> * \<langle>`i \<noteq> 0\<rangle>,
+         EXS A B. llist A i * llist B j * \<langle>rev xs = (rev A) @ B\<rangle>\<rbrakk>
+      od"
       by morgan sep_auto+
   also have "... \<le> 
-      assign j_update $0; 
-      while ({(s, h). i s \<noteq> 0})  (
-        lookup k_update (\<lambda>s. i s + 1);
-        mutation (\<lambda>s. i s + 1) j;
-        (spec (EXS A B a. (i \<mapsto> $a, j) * llist A k * llist B j * <{s. rev xs = (rev (Cons a A)) @ B}> * <{s. i s \<noteq> 0}>)
-              (EXS A B. llist A i * llist B j * <{s. rev xs = (rev A) @ B}>))
-      )"
+      `j := 0; 
+      while `i \<noteq> 0 do 
+        `k := @(`i + 1);
+        @(`i + 1) := `j;
+        \<lbrakk>EXS A B a. (i \<mapsto> $a, j) * llist A k * llist B j * \<langle>rev xs = (rev (a#A)) @ B\<rangle> * \<langle>`i \<noteq> 0\<rangle>,
+         EXS A B. llist A i * llist B j * \<langle>rev xs = (rev A) @ B\<rangle>\<rbrakk>
+      od"
     by morgan
-  also have "... \<le> 
-      assign j_update $0; 
-      while ({(s, h). i s \<noteq> 0})  (
-        lookup k_update (\<lambda>s. i s + 1);
-        mutation (\<lambda>s. i s + 1) j;
-        (spec (EXS A B a. llist A k * (i \<mapsto> $a, j) * llist B j * <{s. rev xs = (rev (Cons a A)) @ B}> * <{s. i s \<noteq> 0}>)
-              (EXS A B. llist A i * llist B j * <{s. rev xs = (rev A) @ B}>))
-      )"
-    by morgan sep_auto
     also have "... \<le> 
-      assign j_update $0; 
-      while ({(s, h). i s \<noteq> 0})  (
-        lookup k_update (\<lambda>s. i s + 1);
-        mutation (\<lambda>s. i s + 1) j;
-        (spec (EXS A B a. llist A k * llist (Cons a B) i * <{s. rev xs = (rev A) @ (Cons a B)}> * <{s. i s \<noteq> 0}>)
-              (EXS A B. llist A i * llist B j * <{s. rev xs = (rev A) @ B}>))
-      )"
-      by morgan sep_auto
-    also have "... \<le> 
-      assign j_update $0; 
-      while ({(s, h). i s \<noteq> 0})  (
-        lookup k_update (\<lambda>s. i s + 1);
-        mutation (\<lambda>s. i s + 1) j;
-        (spec (EXS A B. llist A k * llist B i * <{s. rev xs = (rev A) @ B}> * <{s. i s \<noteq> 0}>)
-              (EXS A B. llist A i * llist B j * <{s. rev xs = (rev A) @ B}>))
-      )"
+      `j := 0; 
+      while `i \<noteq> 0 do 
+        `k := @(`i + 1);
+        @(`i + 1) := `j;
+        \<lbrakk>EXS A B. llist A k * llist B i * \<langle>rev xs = (rev A) @ B\<rangle> * \<langle>`i \<noteq> 0\<rangle>,
+         EXS A B. llist A i * llist B j * \<langle>rev xs = (rev A) @ B\<rangle>\<rbrakk>
+      od"
       by morgan sep_auto+
     also have "... \<le> 
-      assign j_update $0; 
-      while ({(s, h). i s \<noteq> 0})  (
-        lookup k_update (\<lambda>s. i s + 1);
-        mutation (\<lambda>s. i s + 1) j;
-        assign j_update i;
-        (spec (EXS A B. llist A k * llist B j * <{s. rev xs = (rev A) @ B}> * <{s. j s \<noteq> 0}>)
-              (EXS A B. llist A i * llist B j * <{s. rev xs = (rev A) @ B}>))
-      )"
+      `j := 0; 
+      while `i \<noteq> 0 do 
+        `k := @(`i + 1);
+        @(`i + 1) := `j;
+        `j := `i;
+        \<lbrakk>EXS A B. llist A k * llist B j * \<langle>rev xs = (rev A) @ B\<rangle> * \<langle>`j \<noteq> 0\<rangle>,
+         EXS A B. llist A i * llist B j * \<langle>rev xs = (rev A) @ B\<rangle>\<rbrakk>
+      od"
       by morgan sep_auto
     also have "... \<le> 
-      assign j_update $0; 
-      while ({(s, h). i s \<noteq> 0})  (
-        lookup k_update (\<lambda>s. i s + 1);
-        mutation (\<lambda>s. i s + 1) j;
-        assign j_update i;
-        assign i_update k
-      )"
+      `j := 0; 
+      while `i \<noteq> 0 do 
+        `k := @(`i + 1);
+        @(`i + 1) := `j;
+        `j := `i;
+        `i := `k
+      od"
       by morgan sep_auto
     finally show ?thesis .
 qed
 
 
-lemma "ht (llist xs i)(
-      assign j_update $0;
-      awhile (EXS as bs. (llist as i * llist bs j) * (<{s. rev xs = rev as @ bs}>))
-        ({(s, h). i s \<noteq> 0}) 
-        (
-          apre (EXS A B a k. (i \<mapsto> $a, $k) * llist A $k * llist B j * <{s. rev xs = (rev (Cons a A)) @ B}> * <{s. i s \<noteq> 0}>)
-          (lookup k_update (\<lambda>s. i s + 1));
-          apost 
-          (mutation (\<lambda>s. i s + 1) j)
-          ((EXS A B a. (i \<mapsto> $a, j) * llist A k * llist B j * <{s. rev xs = (rev (Cons a A)) @ B}> * <{s. i s \<noteq> 0}>));
-          assign j_update i;
-          assign i_update k
-        )
-      )(llist (rev xs) j)"
-by (hoare; sep_safe) sep_auto+
+lemma "\<turnstile> \<lbrace> list_seg (x#xs) i k \<rbrace>
+      `j := @(`i + 1);
+      dispose `i;
+      dispose (`i + 1);
+      `i := `j
+    \<lbrace> list_seg xs i k \<rbrace>"
+ by hoare sep_auto+
 
+lemma exsI: "(x, y) \<in> (EXS xa xb xc x. P x \<inter> Q xa xb xc x) \<Longrightarrow> (x, y) \<in> (EXS x. P x \<inter> (EXS xa xb xc. Q xa xb xc x))"
+  by auto
+
+lemma deallocI [intro]: "(x, y) \<in> {(s, h). i s \<noteq> 0} \<Longrightarrow>
+              (x, y) \<in> llist xa i \<Longrightarrow>
+              (x, y) \<in> (EXS x. ((\<lambda>s. i (s\<lparr>j := i s\<rparr>) + 1) \<mapsto> (\<lambda>s. x)) * true \<inter> (EXS xa xb xc. ((\<lambda>s. j (s\<lparr>j := i s, i := x\<rparr>)) \<mapsto> (\<lambda>s. xa)) * (((\<lambda>s. j (s\<lparr>j := i s, i := x\<rparr>) + 1) \<mapsto> (\<lambda>s. xb)) * llist xc (\<lambda>s. i (s\<lparr>j := i s, i := x\<rparr>)))))"
+  apply (rule exsI)
+  apply safe
+  apply (drule llist_cons) back
+  apply assumption
+  apply auto
+  apply (rule_tac x="hd xa" in exI)
+  apply (rule_tac x=j in exI)
+  apply (rule_tac x="tl xa" in exI)
+  apply (rule_tac x=j in exI)
+  apply auto
+by (metis (no_types, lifting) bbi.Sup.qisol bbi.mult.left_commute contra_subsetD top_greatest)
+
+lemma "\<turnstile> \<lbrace> llist xs i \<rbrace>
+      while `i \<noteq> 0 
+      inv EXS ys. llist ys i 
+      do
+        `j := `i;
+        `i := @(`i + 1);
+        dispose `j;
+        dispose (`j + 1)
+      od
+    \<lbrace> emp \<rbrace>"
+by hoare (sep_safe, (rule deallocI, auto | sep_auto))+
+
+declare sl_frame [sl]
+
+lemma "\<turnstile> \<lbrace> llist xs i \<rbrace>
+      `j := 0;
+      while `i \<noteq> 0 
+      inv EXS as bs. (llist as i * llist bs j) * \<langle>rev xs = rev as @ bs\<rangle>
+      do
+        \<lbrace> EXS A B a k. (i \<mapsto> $a, $k) * llist A $k * llist B j * \<langle>rev xs = (rev (a#A)) @ B\<rangle> * \<langle>`i \<noteq> 0\<rangle> \<rbrace>
+        `k := @(`i + 1); 
+        @(`i + 1) := `j
+        \<lbrace> EXS A B a. (i \<mapsto> $a, j) * llist A k * llist B j * \<langle>rev xs = (rev (a#A)) @ B\<rangle> * \<langle>`i \<noteq> 0\<rangle> \<rbrace>;
+        `j := `i;
+        `i := `k
+      od
+      \<lbrace> llist (rev xs) j \<rbrace>"
+by (hoare; sep_safe) sep_auto+
 
 end
